Graphiti/Core/Rewrites/Fork8Rewrite.lean
@@ -1,5 +1,5 @@
 /-
-Copyright (c) 2024, 2025 VCA Lab, EPFL. All rights reserved.
+Copyright (c) 2024-2025 VCA Lab, EPFL. All rights reserved.
 Released under Apache 2.0 license as described in the file LICENSE.
 Authors: Ayatallah Elakhras, Yann Herklotz
 -/
@@ -11,21 +11,17 @@ namespace Graphiti.Fork8Rewrite
 
 open StringModule
 
-def matcher (g : ExprHigh String String) : RewriteResult (List String × List String) := do
+def matcher : Pattern String (String × Nat) 1 := fun g => do
   let (.some list) ← g.modules.foldlM (λ s inst (pmap, typ) => do
       if s.isSome then return s
 
-      unless "fork".isPrefixOf typ do return none
+      unless "fork8" == typ.1 do return none
 
-      let l := typ.splitOn " "
-      unless l.getLast? = .some "8" do return none
-      let forkType := l.drop 1 |>.dropLast |> " ".intercalate
-
-      return some ([inst], [forkType])
+      return some ([inst], #v[typ.2])
     ) none | throw .done
   return list
 
-def lhs (T : Type) (Tₛ : String) : ExprHigh String String × IdentMap String (TModule1 String) := [graphEnv|
+def lhs (types : Vector Nat 1) : ExprHigh String (String × Nat) := [graph|
     i [type = "io"];
     o1 [type = "io"];
     o2 [type = "io"];
@@ -36,7 +32,7 @@ def lhs (T : Type) (Tₛ : String) : ExprHigh String String × IdentMap String (
     o7 [type = "io"];
     o8 [type = "io"];
 
-    fork [typeImp = $(⟨_, fork T 8⟩), type = $("fork " ++ Tₛ ++ " 8")];
+    fork [type = "fork8", arg = $(types[0])];
 
     i -> fork [to="in1"];
     fork -> o1 [from="out1"];
@@ -49,15 +45,13 @@ def lhs (T : Type) (Tₛ : String) : ExprHigh String String × IdentMap String (
     fork -> o8 [from="out8"];
   ]
 
-def lhs_extract T₁ := (lhs Unit T₁).fst.extract ["fork"] |>.get rfl
-
-theorem lhs_type_independent a c T₁ : (lhs a T₁).fst = (lhs c T₁).fst := by rfl
+def lhs_extract T₁ := (lhs T₁).extract ["fork"] |>.get rfl
 
 theorem double_check_empty_snd T₁ : (lhs_extract T₁).snd = ExprHigh.mk ∅ ∅ := by rfl
 
 def lhsLower T₁ := lhs_extract T₁ |>.fst.lower.get rfl
 
-def rhs (T : Type) (Tₛ : String) : ExprHigh String String × IdentMap String (TModule1 String) := [graphEnv|
+def rhs (m : Nat) : ExprHigh String (String × Nat) := [graph|
     i [type = "io"];
     o1 [type = "io"];
     o2 [type = "io"];
@@ -68,8 +62,8 @@ def rhs (T : Type) (Tₛ : String) : ExprHigh String String × IdentMap String (
     o7 [type = "io"];
     o8 [type = "io"];
 
-    fork1 [typeImp = $(⟨_, fork T 2⟩), type = $("fork " ++ Tₛ ++ " 2")];
-    fork2 [typeImp = $(⟨_, fork T 7⟩), type = $("fork " ++ Tₛ ++ " 7")];
+    fork1 [type = $("fork2"), arg = $(m+1)];
+    fork2 [type = $("fork7"), arg = $(m+2)];
 
     i -> fork1 [to="in1"];
     fork1 -> fork2 [from="out2", to="in1"];
@@ -84,21 +78,21 @@ def rhs (T : Type) (Tₛ : String) : ExprHigh String String × IdentMap String (
     fork2 -> o8 [from="out7"];
   ]
 
-def rhs_extract S₁ := (rhs Unit S₁).fst.extract ["fork1", "fork2"] |>.get rfl
+def rhs_extract S₁ := (rhs S₁).extract ["fork1", "fork2"] |>.get rfl
 
 def rhsLower T₁ := (rhs_extract T₁).fst.lower.get rfl
 
-theorem rhs_type_independent a c T₁ : (rhs a T₁).fst = (rhs c T₁).fst := by rfl
+def findRhs mod := (rhs_extract 0).fst.modules.find? mod |>.map Prod.fst
 
-def findRhs mod := (rhs_extract "").fst.modules.find? mod |>.map Prod.fst
-
-def rewrite : Rewrite String String :=
-  { abstractions := [],
-    pattern := matcher,
-    rewrite := λ | [T₁] => pure ⟨lhsLower T₁, rhsLower T₁⟩ | _ => failure
+def rewrite : Rewrite String (String × Nat) :=
+  { abstractions := []
+    params := 1
+    pattern := matcher
+    rewrite := λ l m => ⟨lhsLower l, rhsLower m⟩
     name := .some "fork-8"
     transformedNodes := [.none]
     addedNodes := [findRhs "fork1" |>.get rfl, findRhs "fork2" |>.get rfl]
+    fresh_types := 2
   }
 
 end Graphiti.Fork8Rewrite
