Graphiti/Core/Rewrites/JoinSplitLoopCond.lean
@@ -1,7 +1,7 @@
 /-
-Copyright (c) 2024 VCA Lab, EPFL. All rights reserved.
+Copyright (c) 2024-2025 VCA Lab, EPFL. All rights reserved.
 Released under Apache 2.0 license as described in the file LICENSE.
-Authors: Ayatallah Elakhras
+Authors: Ayatallah Elakhras, Yann Herklotz
 -/
 
 import Graphiti.Core.Rewriter
@@ -11,39 +11,42 @@ namespace Graphiti.JoinSplitLoopCond
 
 open StringModule
 
+variable (T : Vector Nat 3)
+variable (M : Nat)
+
 -- Search for a fork Bool 2 that feeds an Init and a Branch
-def matcher (g : ExprHigh String String) : RewriteResult (List String × List String) := do
+def matcher : Pattern String (String × Nat) 3 := fun g => do
   let (.some list) ← g.modules.foldlM (λ s inst (pmap, typ) => do
       if s.isSome then return s
-        unless typ = "init Bool false" do return none
+        unless typ.1 == "initBool" do return none
 
       let (.some condFork) := followInput g inst "in1" | return none
-      unless condFork.typ = "fork Bool 2" do return none
+      unless condFork.typ.1 == "fork2" do return none
 
       -- Make sure that the input of the fork is not a split; otherwise, the matcher will apply forever
       let (.some genericInFork) := followInput g condFork.inst "in1" | return none
 
       let (.some branch) := followOutput g condFork.inst "out1" | return none
-      unless String.isPrefixOf "branch" branch.typ && branch.inputPort = "in2" do return none
+      unless "branch" == branch.typ.1 && branch.inputPort = "in2" do return none
 
       let (.some genericInBranch) := followInput g branch.inst "in1" | return none
 
       unless ¬(genericInBranch.inst == genericInFork.inst) do return none
 
-      return ([branch.inst, inst, condFork.inst], [extractType branch.typ, extractType branch.typ])
+      return ([branch.inst, inst, condFork.inst], #v[branch.typ.2, typ.2, condFork.typ.2])
     ) none | MonadExceptOf.throw RewriteError.done
   return list
 
-def lhs (T T' : Type) (Tₛ T'ₛ : String) : ExprHigh String String × IdentMap String (TModule1 String) := [graphEnv|
+def lhs : ExprHigh String (String × Nat) := [graph|
     d_i [type = "io"];
     c_i [type = "io"];
     o_br_t [type = "io"];
     o_br_f [type = "io"];
     o_init [type = "io"];
 
-    branch [typeImp = $(⟨_, branch T⟩), type = $("branch " ++ Tₛ)];
-    condFork [typeImp = $(⟨_, fork Bool 2⟩), type = "fork Bool 2"];
-    init [typeImp = $(⟨_, init Bool false⟩), type = "init Bool false"];
+    branch [type = "branch", arg = $(T[0])];
+    condFork [type = "fork2", arg = $(T[1])];
+    init [type = "initBool", arg = $(T[2])];
 
     c_i -> condFork [to="in1"];
     d_i -> branch [to="in1"];
@@ -55,49 +58,24 @@ def lhs (T T' : Type) (Tₛ T'ₛ : String) : ExprHigh String String × IdentMap
     init -> o_init [from = "out1"];
   ]
 
-def lhs' (T T' : Type) (Tₛ T'ₛ : String) : ExprHigh String String × IdentMap String (TModule1 String) := [graphEnv|
+def lhs_extract := (lhs T).extract ["branch", "init", "condFork"] |>.get rfl
+
+theorem double_check_empty_snd : (lhs_extract T).snd = ExprHigh.mk ∅ ∅ := by rfl
+
+def lhsLower := lhs_extract T |>.fst.lower.get rfl
+
+def rhs : ExprHigh String (String × Nat) := [graph|
     d_i [type = "io"];
     c_i [type = "io"];
     o_br_t [type = "io"];
     o_br_f [type = "io"];
     o_init [type = "io"];
 
-    branch [typeImp = $(⟨_, branch T⟩), type = $("branch " ++ Tₛ)];
-    condFork [typeImp = $(⟨_, fork Bool 2⟩), type = "fork Bool 2"];
-    init [typeImp = $(⟨_, init Bool false⟩), type = "init Bool false"];
-
-    c_i -> condFork [to="in1"];
-    d_i -> branch [to="in1"];
-    condFork -> branch [from="out1", to="in2"];
-    condFork -> init [from="out2", to="in1"];
-
-    branch -> o_br_t [from = "out1"];
-    branch -> o_br_f [from = "out2"];
-    init -> o_init [from = "out1"];
-  ]
-
-def lhs_extract T₁ T₂ := (lhs Unit Unit T₁ T₂).fst.extract ["branch", "init", "condFork"] |>.get rfl
-
--- #eval IO.print ((lhs Unit Unit "T" "T'").fst)
-
-theorem lhs_type_independent a b c d T₁ T₂ : (lhs a b T₁ T₂).fst = (lhs c d T₁ T₂).fst := by rfl
-
-theorem double_check_empty_snd T₁ T₂ : (lhs_extract T₁ T₂).snd = ExprHigh.mk ∅ ∅ := by rfl
-
-def lhsLower T₁ T₂ := lhs_extract T₁ T₂ |>.fst.lower.get rfl
-
-def rhs (T T' : Type) (Tₛ Tₛ' : String) : ExprHigh String String × IdentMap String (TModule1 String) := [graphEnv|
-    d_i [type = "io"];
-    c_i [type = "io"];
-    o_br_t [type = "io"];
-    o_br_f [type = "io"];
-    o_init [type = "io"];
-
-    branch [typeImp = $(⟨_, branch T⟩), type = $("branch " ++ Tₛ)];
-    condFork [typeImp = $(⟨_, fork Bool 2⟩), type = "fork Bool 2"];
-    init [typeImp = $(⟨_, init Bool false⟩), type = "init Bool false"];
-    join [typeImp = $(⟨_, join T Bool⟩), type = $("join " ++ Tₛ ++ " Bool")];
-    split [typeImp = $(⟨_, split T Bool⟩), type = $("split " ++ Tₛ ++ " Bool")];
+    branch [type = "branch", arg = $(M+1)];
+    condFork [type = "fork2", arg = $(M+2)];
+    init [type = "initBool", arg = $(M+3)];
+    join [type = "join", arg = $(M+4)];
+    split [type = "split", arg = $(M+5)];
 
     d_i -> join [to="in1"];
     c_i -> join [to="in2"];
@@ -115,20 +93,21 @@ def rhs (T T' : Type) (Tₛ Tₛ' : String) : ExprHigh String String × IdentMap
     init -> o_init [from = "out1"];
   ]
 
-def rhsLower T₁ T₂ := (rhs Unit Unit T₁ T₂).fst.lower.get rfl
+def rhs_extract := (rhs M).extract ["branch", "condFork", "init", "join", "split"] |>.get rfl
 
--- #eval IO.print ((rhs Unit Unit "T" "T'").fst)
+def rhsLower := (rhs M).lower.get rfl
 
-theorem rhs_type_independent a b c d T₁ T₂ : (rhs a b T₁ T₂).fst = (rhs c d T₁ T₂).fst := by rfl
+def findRhs mod := (rhs_extract 0).fst.modules.find? mod |>.map Prod.fst
 
-def rewrite : Rewrite String String :=
+def rewrite : Rewrite String (String × Nat) :=
   { abstractions := [],
+    params := 3
     pattern := matcher,
-    rewrite := λ l => do
-      let T₁ ← l[0]?
-      let T₂ ← l[1]?
-      return ⟨ lhsLower T₁ T₂, rhsLower T₁ T₂ ⟩
+    rewrite := λ l n => ⟨ lhsLower l, rhsLower n ⟩
     name := .some "join-split-loop-cond"
+    transformedNodes := [findRhs "branch", findRhs "init", findRhs "condFork"]
+    addedNodes := [findRhs "join" |>.get rfl, findRhs "split" |>.get rfl]
+    fresh_types := 5
   }
 
 end Graphiti.JoinSplitLoopCond
